#Теорема 
#Доказательство 
Для [[Мультипликативная группа|мултипликативных групп]]:
$$
\forall m,n \in \mathbb{Z}
$$
$$
a^{m}a^{n}=a^{m+n} \wedge (a^{m})^{n} = a^{mn}
$$
Для [[Аддитивная группа|аддитивных групп]]:
$$
ma+na=(m+n)a \wedge n(ma)=(nm)a
$$

### Доказательство
1. $m \geq 0$, $n \geq 0$
$a^{m}a^{m}=$
$(a*\dots*a(m \text{ раз})) * (a*\dots*a(n \text{ раз}))=a^{m+n}$

2. $m < 0, n > 0$
Пусть $m'=-m>0, n<0$
$a^{m}a^{m}=$
$(a^{-1}*\dots*a^{-1}(m \text{ раз})) * (a*\dots*a(n \text{ раз}))=$
$=a^{m'-n}=a^{m+n}(n>m)$

3. $m>0, n<0$ аналогично п.2
4. $m<0,n>0$ аналогично п.1
